Lemmas with substitutions

src/Compatibility.v
@@ -76,13 +76,168 @@ Qed.
 
 Lemma subst_composition :
   forall e ξ l vals Γ, length l = length vals -> subscoped Γ [] ξ ->
+  EXP Γ ++ l ⊢ e ->
   composition (subst (idsubst[[ ::= combine l vals]])) (subst (ξ -- l)) e = subst (ξ[[::= combine l vals]]) e.
 Proof.
   induction e; intros; unfold composition; simpl; auto.
   * unfold "--". simpl. destruct (in_list (inl v) l) eqn:P.
     - simpl. apply subst_list_in; auto. apply in_list_sound in P. auto. 
-    - apply not_in_list_sound in P. rewrite subst_list_not_in; auto. unfold subscoped in H0.
-      rewrite subst_list_not_in.
+    - inversion H1. inversion H2. subst. apply not_in_list_sound in P.
+      apply in_app_iff in H5. destruct H5. 2: contradiction.
+      rewrite subst_list_not_in; auto.
+      specialize (H0 _ H3). eapply vclosed_ignores_sub in H0. rewrite H0. reflexivity.
+  * unfold "--". simpl. destruct (in_list (inr f) l) eqn:P.
+    - simpl. apply subst_list_in; auto. apply in_list_sound in P. auto. 
+    - inversion H1. inversion H2. subst. apply not_in_list_sound in P.
+      apply in_app_iff in H5. destruct H5. 2: contradiction.
+      rewrite subst_list_not_in; auto.
+      specialize (H0 _ H3). eapply vclosed_ignores_sub in H0. rewrite H0. reflexivity.
+  * assert ((subst ((idsubst [[ ::= combine l vals]]) -- map inl vl) (subst ((ξ -- l) -- map inl vl) e)) = (subst ((ξ [[ ::= combine l vals]]) -- map inl vl) e)).
+    { unfold composition in IHe.
+Abort.
+
+Definition varname (e : Exp) : option VarFunId :=
+match e with
+| EVar v   => Some (inl v)
+| EFunId f => Some (inr f)
+| _        => None
+end.
+
+Definition substcomp (ξ η : Substitution) : Substitution :=
+  composition (subst ξ) η.
+(* fun x =>
+  match (varname (η x)) with
+  | Some vname => ξ vname
+    (* if var_funid_eqb vname x
+    then ξ x
+    else η x *)
+  | _ => η x
+end. *)
+(* 
+Lemma idsubst_varname : forall x, varname (idsubst x) = Some x.
+Proof.
+  intros. destruct x; cbn; auto.
+Qed.
+*)
+
+Lemma subst_restrict_app :
+  forall ξ l1 l2, ((ξ -- l1) -- l2) = (ξ -- (l1 ++ l2)).
+Proof.
+  intros. extensionality x. unfold "--". break_match_goal.
+  * apply in_list_sound in Heqb. eapply in_app_right in Heqb.
+    apply in_list_sound in Heqb. rewrite Heqb. auto.
+  * break_match_goal.
+    - apply in_list_sound in Heqb0. eapply in_app_left in Heqb0.
+      apply in_list_sound in Heqb0. rewrite Heqb0. auto.
+    - apply not_in_list_sound in Heqb. apply not_in_list_sound in Heqb0.
+      eapply app_not_in in Heqb; eauto. apply not_in_list_sound in Heqb. rewrite Heqb. auto.
+Qed.
+
+Lemma subst_composition :
+  forall e ξ η l,
+  (subst (η[[::= l]])) (subst (ξ -- fst (split l)) e) = 
+  subst (substcomp (η[[::= l]]) (ξ -- fst (split l))) e.
+Proof.
+  induction e; intros; auto; simpl.
+  * Search "--". rewrite subst_restrict_app.
+Abort.
+
+(** In general, the following lemma could not be weakened more:
+    (ξ₁ -- l) cannot be replaced by ξ₁ on the right-hand side.
+*)
+Lemma substcomp_restrict : forall ξ₁ ξ₂ l,
+  (substcomp (ξ₁ -- l) (ξ₂ -- l)) = (substcomp (ξ₁ -- l) ξ₂ -- l).
+Proof.
+  intros. unfold "--". extensionality x.
+  break_match_goal; cbn.
+  * rewrite Heqb. destruct x; simpl; break_match_goal; auto.
+    - apply in_list_sound in Heqb. apply not_in_list_sound in Heqb0. contradiction. (* Coq bug *)
+    - apply in_list_sound in Heqb. apply not_in_list_sound in Heqb0. contradiction.
+  * rewrite Heqb. unfold substcomp, composition. reflexivity.
+Qed.
+
+(*
+    What if ξ₂ produced closed values? Or just ξ₂'s result is NOT containing any
+    variables of l?
+*)
+Lemma substcomp_restrict_x : forall ξ₁ ξ₂ l x, VALCLOSED (ξ₂ x) ->
+  (substcomp (ξ₁ -- l) (ξ₂ -- l)) x = (substcomp ξ₁ ξ₂ -- l) x.
+Proof.
+  intros. rewrite substcomp_restrict. unfold substcomp, "--", composition.
+  break_match_goal; auto.
+  eapply vclosed_ignores_sub in H as H'. rewrite H'.
+  eapply vclosed_ignores_sub in H. rewrite H. auto.
+Qed.
+
+Corollary substcomp_restrict_subscoped : forall e ξ₁ ξ₂ l Γ, subscoped Γ [] ξ₂ ->
+  EXP Γ ⊢ e ->
+  subst (substcomp (ξ₁ -- l) (ξ₂ -- l)) e = subst (substcomp ξ₁ ξ₂ -- l) e.
+Proof.
+  induction e; intros; simpl; auto.
+  * apply substcomp_restrict_x. apply H. inversion H0. inversion H1. auto.
+  * apply substcomp_restrict_x. apply H. inversion H0. inversion H1. auto.
+  *
+Abort.
+
+(**
+  with capture-avoiding substitution, this should be trivial
+*)
+Lemma subst_composition2 :
+  forall e ξ₁ ξ₂ , (* Γ, subscoped Γ [] ξ₁ -> subscoped Γ [] ξ₂ ->
+  EXP Γ ⊢ e ->*)
+  (subst ξ₁) (subst ξ₂ e) = subst (substcomp ξ₁ ξ₂) e.
+Proof.
+  induction e; intros; simpl; auto.
+  * erewrite IHe, substcomp_restrict.
+Abort.
+
+Lemma subst_composition_scoped :
+  forall ξ η Γ Γ', subscoped Γ Γ' ξ -> subscoped Γ Γ' η -> subscoped Γ Γ' (substcomp ξ η).
+Proof.
+  intros. intro. intros. unfold substcomp. break_match_goal;
+  [ apply H | apply H0 ]; auto.
+  
+Qed.
+
+Lemma subst_list_in_val : forall l x vals ξ, length l = length vals ->
+  In x l -> exists v, In v vals /\ (ξ[[ ::= combine l vals]]) x = v.
+Proof.
+  induction l; intros.
+  * inversion H0.
+  * apply element_exist in H as H0'. destruct H0', H1. subst. inversion H.
+    unfold extend_subst. destruct (in_dec var_funid_eq_dec x l).
+    - epose (IHl x x1 _ H2 i). destruct e, H1. exists x2. split. firstorder.
+      simpl. eexact H3.
+    - inversion H0. 2: contradiction. subst.
+      exists x0. split. firstorder. simpl.
+      repeat rewrite subst_list_not_in; auto.
+      unfold extend_subst. rewrite var_funid_eqb_refl. auto.
+Qed.
+
+Lemma subscoped_ext_app :
+  forall ξ Γ Γ' l vals, subscoped Γ Γ' ξ -> length l = length vals ->
+  Forall (fun v => VAL Γ' ⊢ v ) vals ->
+  subscoped (Γ ++ l) Γ' (substcomp (idsubst[[::= combine l vals]]) (ξ -- l)).
+Proof.
+  intros. intro. intros. unfold "--", substcomp. break_match_goal.
+  * break_match_hyp.
+    - apply in_list_sound in Heqb. Check subst_list_in.
+      epose (subst_list_in_val _ _ _ _ H0 Heqb). destruct e. destruct H3.
+      rewrite H4. rewrite indexed_to_forall in H1. (* Just technical, but doable *)
+Admitted.
+
+Lemma biforall_vrel_helper : forall m vals1 vals2, length vals1 = length vals2 ->
+  list_biforall (Vrel m) vals1 vals2 ->
+  Forall (fun v : Exp => VALCLOSED v) vals1 /\
+  Forall (fun v : Exp => VALCLOSED v) vals2.
+Proof.
+  induction vals1; intros.
+  * apply eq_sym, length_zero_iff_nil in H. subst. firstorder.
+  * apply element_exist in H as H'. destruct H', H1. subst. inversion H.
+    inversion H0. subst. apply Vrel_closed in H5. destruct H5.
+    split; constructor; auto.
+    - apply (IHvals1 x0); auto.
+    - apply (IHvals1 x0); auto.
 Qed.
 
 Lemma Vrel_Fun_compat :
@@ -96,7 +251,13 @@ Proof.
   - constructor. eapply subst_preserves_scope_rev; eauto. eapply Erel_open_scope in H. apply H.
   - constructor. eapply subst_preserves_scope_rev; eauto. eapply Erel_open_scope in H. apply H.
   - break_match_goal; try congruence. intros. unfold Erel_open in H.
+    Search subst.
+    rewrite subst_composition; eauto.
     unfold Erel in H.
-     eapply H.
-Qed.
-
+    eapply H. unfold Grel. split. 2: split.
+    1-2: apply subscoped_ext_app; auto.
+    1, 3: rewrite map_length; auto.
+    1-2: apply biforall_vrel_helper in H6.
+    1-4: try lia; destruct H6; auto.
+    intros. unfold substcomp. (* Technical, but doable *)
+Admitted.
